# baseURI: https://www.w3.org/2006/time/ng
# imports: http://purl.org/dc/elements/1.1/
# imports: http://www.w3.org/2006/time

@prefix dct: <http://purl.org/dc/terms/> .
@prefix owl: <http://www.w3.org/2002/07/owl#> .
@prefix rdf: <http://www.w3.org/1999/02/22-rdf-syntax-ns#> .
@prefix rdfs: <http://www.w3.org/2000/01/rdf-schema#> .
@prefix skos: <http://www.w3.org/2004/02/skos/core#> .
@prefix time: <http://www.w3.org/2006/time#> .
@prefix xsd: <http://www.w3.org/2001/XMLSchema#> .

time:Era
  a owl:Class ;
  rdfs:label "Era"@en ;
  skos:definition """A linear (non-cyclic) year numbering system. 
No assumption is made with regards to the details of how years are numbered in the era, such as a year 0, or years with negative indexes.
Any year numbering system can be an instance of this class even if the year definition doesn't match the one of the Gregorian calendar.
For instance Roman regnal years or Chinese eras can be encoded as instances of :Era.

An era can correspond to a temporal entity (ex: a Roman Emperor reign) but does not have to (for instance the Common Era which does not have bounds for its beginning or end)."""@en ;
  skos:example """
ex:KaliYugaEra
  a time:Era ;
  rdfs:label \"Kali Yuga\"@en ;
.""" ;
.
time:era
  a owl:ObjectProperty ;
  rdfs:domain time:GeneralDateTimeDescription ;
  rdfs:label "in era"@en ;
  rdfs:range time:Era ;
  skos:definition "Era indication"@en ;
  skos:example """
ex:TwentyTwenty
  a time:GeneralDateTimeDescription ;
  time:year "5121"^^time:generalYear ;
  time:era ex:KaliYuga ;
.""" ;
.
time:reignOf
  a owl:ObjectProperty ;
  rdfs:domain time:Era ;
  rdfs:label "in reign of"@en ;
  skos:definition """Indicates the person whose reign is associated with the era.
Most eras are assciated with one reign (ex: Roman regnal years), but sometimes several eras are associated with one reign (ex: later Chinese eras).
This property can be used in both cases.
No range is indicated so that the associated person can have any relevant type."""@en ;
  skos:example """
ex:DiocletianRegnalYears
  a time:Era ;
  time:reignOf ex:Diocletian ;
.""" ;
.
time:CommonEra a time:Era ;
  rdfs:label "Common Era"@en ;
  skos:definition """The Era of the modern gregorian calendar. It is defined so that a general year in a date object associated with this era is roughly equivalent to a gYear.

This specification doesn't say anything about the general year being a year of the gregorian calendar, so any type of year can be used.
For example, a date in the Chinese calendar may be given using a year indicated in the Common Era, even though the Chinese year starts and ends after the one of the Gregorian calendar.
This means that 

ex:Date1
  "xxx"^^:generalYear ;
  :era :CommonEra ;
.
should not be considered equivalent to

ex:Date1
  "xxx"^^xsd:gYear ;
."""@en ;
.
<https://www.w3.org/2006/time/era>
  a owl:Ontology ;
  dct:created "2020-07-10"^^xsd:date ;
  dct:creator <https://orcid.org/0000-0002-3787-8226> ;
  dct:license <https://creativecommons.org/share-your-work/public-domain/cc0/> ;
  dct:modified "2020-07-10"^^xsd:date ;
  rdfs:comment "An extension of OWL-Time allowing encoding of eras"@en ;
  rdfs:label "OWL-Time Era extensions" ;
  owl:imports <http://www.w3.org/2006/time> ;
.